src/mqtt-packet-parser/src/disconnect.fst
@@ -5,8 +5,11 @@ open C.String
 open Const
 open Common
 open FStar.HyperStack.ST
+open LowStar.BufferOps
 
 module U8 = FStar.UInt8
+module U16 = FStar.UInt16
+module U32 = FStar.UInt32
 module B = LowStar.Buffer
 
 val assemble_disconnect_struct: s: struct_disconnect_parts
@@ -49,130 +52,172 @@ let assemble_disconnect_struct s =
       publish = {
         topic_length = 0ul;
         topic_name = !$"";
+        packet_identifier = max_u16;
         property_length = 0ul;
         payload = !$"";
         payload_length = 0ul;
         property_id = max_u8;
       };
-      disconnect = (
-        if (U8.eq disconnect_constant.flags_constant.flag define_disconnect_reason_code_normal_disconnection) then
-          define_struct_disconnect_normal_disconnection
-
-        else if (U8.eq disconnect_constant.flags_constant.flag define_disconnect_reason_code_disconnect_with_will_message) then
-          define_struct_disconnect_disconnect_with_will_message
-
-        else if (U8.eq disconnect_constant.flags_constant.flag define_disconnect_reason_code_unspecified_error) then
-          define_struct_disconnect_unspecified_error
-
-        else if (U8.eq disconnect_constant.flags_constant.flag define_disconnect_reason_code_malformed_packet) then
-          define_struct_disconnect_malformed_packet
-
-        else if (U8.eq disconnect_constant.flags_constant.flag define_disconnect_reason_code_protocol_error) then
-          define_struct_disconnect_protocol_error
-
-        else if (U8.eq disconnect_constant.flags_constant.flag define_disconnect_reason_code_implementation_specific_error) then
-          define_struct_disconnect_implementation_specific_error
-
-        else if (U8.eq disconnect_constant.flags_constant.flag define_disconnect_reason_code_not_authorized) then
-          define_struct_disconnect_not_authorized
-
-        else if (U8.eq disconnect_constant.flags_constant.flag define_disconnect_reason_code_server_busy) then
-          define_struct_disconnect_server_busy
-
-        else if (U8.eq disconnect_constant.flags_constant.flag define_disconnect_reason_code_server_shutting_down) then
-          define_struct_disconnect_server_shutting_down
-
-        else if (U8.eq disconnect_constant.flags_constant.flag define_disconnect_reason_code_keep_alive_timeout) then
-            define_struct_disconnect_keep_alive_timeout
-
-        else if (U8.eq disconnect_constant.flags_constant.flag define_disconnect_reason_code_session_taken_over) then
-            define_struct_disconnect_session_taken_over
-            
-        else if (U8.eq disconnect_constant.flags_constant.flag define_disconnect_reason_code_topic_filter_invalid) then
-            define_struct_disconnect_topic_filter_invalid
-        else if (U8.eq disconnect_constant.flags_constant.flag define_disconnect_reason_code_topic_name_invalid) then
-            define_struct_disconnect_topic_name_invalid
-
-        else if (U8.eq disconnect_constant.flags_constant.flag define_disconnect_reason_receive_maximum_exceeded) then
-            define_struct_disconnect_receive_maximum_exceeded
-
-        else if (U8.eq disconnect_constant.flags_constant.flag define_disconnect_reason_topic_alias_invalid) then
-            define_struct_disconnect_topic_alias_invalid
-
-        else if (U8.eq disconnect_constant.flags_constant.flag define_disconnect_reason_packet_too_large) then
-            define_struct_disconnect_packet_too_large
-
-        else if (U8.eq disconnect_constant.flags_constant.flag define_disconnect_reason_message_rate_too_high) then
-            define_struct_disconnect_message_rate_too_high
-
-        else if (U8.eq disconnect_constant.flags_constant.flag define_disconnect_reason_quota_exceeded) then
-            define_struct_disconnect_quota_exceeded
-
-        else if (U8.eq disconnect_constant.flags_constant.flag define_disconnect_reason_administrative_action) then
-            define_struct_disconnect_administrative_action
-
-        else if (U8.eq disconnect_constant.flags_constant.flag define_disconnect_reason_payload_format_invalid) then
-            define_struct_disconnect_payload_format_invalid
-
-        else if (U8.eq disconnect_constant.flags_constant.flag define_disconnect_reason_retain_not_supported) then
-            define_struct_disconnect_retain_not_supported
-
-        else if (U8.eq disconnect_constant.flags_constant.flag define_disconnect_reason_qos_not_supported) then
-            define_struct_disconnect_qos_not_supported
-
-        else if (U8.eq disconnect_constant.flags_constant.flag define_disconnect_reason_use_another_server) then
-            define_struct_disconnect_use_another_server
-
-        else if (U8.eq disconnect_constant.flags_constant.flag define_disconnect_reason_server_moved) then
-            define_struct_disconnect_server_moved
-
-        else if (U8.eq disconnect_constant.flags_constant.flag define_disconnect_reason_shared_subscriptions_not_supported) then
-            define_struct_disconnect_shared_subscriptions_not_supported
-
-        else if (U8.eq disconnect_constant.flags_constant.flag define_disconnect_reason_connection_rate_exceeded) then
-            define_struct_disconnect_connection_rate_exceeded
-
-        else if (U8.eq disconnect_constant.flags_constant.flag define_disconnect_reason_maximum_connect_time) then
-            define_struct_disconnect_maximum_connect_time
-
-        else if (U8.eq disconnect_constant.flags_constant.flag define_disconnect_reason_subscription_identifiers_not_supported) then
-            define_struct_disconnect_subscription_identifiers_not_supported
-
-        else // if (U8.eq disconnect_constant.flags_constant.flag define_disconnect_reason_wildcard_subscriptions_not_supported) then
-            define_struct_disconnect_wildcard_subscriptions_not_supported
-      );
-      property = property_struct_base;
+      disconnect = s.disconnect_struct;
+      property = s.property;
       error = {
         code = define_no_error_code;
         message = define_no_error;
       };
     }
 
+val get_disconnect_reason: reason_code: type_disconnect_reason_code 
+  -> Stack (disconnect_reason_struct: struct_disconnect_reason)
+    (requires fun h0 -> true)
+    (ensures fun h0 r h1 -> true)
+let get_disconnect_reason reason_code =
+  let disconnect_reason_struct: struct_disconnect_reason =
+    (
+      if (U8.eq reason_code define_disconnect_reason_code_normal_disconnection) then
+        define_struct_disconnect_normal_disconnection
+      else if (U8.eq reason_code define_disconnect_reason_code_disconnect_with_will_message) then
+        define_struct_disconnect_disconnect_with_will_message
+      else if (U8.eq reason_code define_disconnect_reason_code_unspecified_error) then
+        define_struct_disconnect_unspecified_error
+      else if (U8.eq reason_code define_disconnect_reason_code_malformed_packet) then
+        define_struct_disconnect_malformed_packet
+      else if (U8.eq reason_code define_disconnect_reason_code_protocol_error) then
+        define_struct_disconnect_protocol_error
+      else if (U8.eq reason_code define_disconnect_reason_code_implementation_specific_error) then
+        define_struct_disconnect_implementation_specific_error
+      else if (U8.eq reason_code define_disconnect_reason_code_not_authorized) then
+        define_struct_disconnect_not_authorized
+      else if (U8.eq reason_code define_disconnect_reason_code_server_busy) then
+        define_struct_disconnect_server_busy
+      else if (U8.eq reason_code define_disconnect_reason_code_server_shutting_down) then
+        define_struct_disconnect_server_shutting_down
+      else if (U8.eq reason_code define_disconnect_reason_code_keep_alive_timeout) then
+        define_struct_disconnect_keep_alive_timeout
+      else if (U8.eq reason_code define_disconnect_reason_code_session_taken_over) then
+        define_struct_disconnect_session_taken_over
+      else if (U8.eq reason_code define_disconnect_reason_code_topic_filter_invalid) then
+        define_struct_disconnect_topic_filter_invalid
+      else if (U8.eq reason_code define_disconnect_reason_code_topic_name_invalid) then
+        define_struct_disconnect_topic_name_invalid
+      else if (U8.eq reason_code define_disconnect_reason_receive_maximum_exceeded) then
+        define_struct_disconnect_receive_maximum_exceeded
+      else if (U8.eq reason_code define_disconnect_reason_topic_alias_invalid) then
+        define_struct_disconnect_topic_alias_invalid
+      else if (U8.eq reason_code define_disconnect_reason_packet_too_large) then
+        define_struct_disconnect_packet_too_large
+      else if (U8.eq reason_code define_disconnect_reason_message_rate_too_high) then
+        define_struct_disconnect_message_rate_too_high
+      else if (U8.eq reason_code define_disconnect_reason_quota_exceeded) then
+        define_struct_disconnect_quota_exceeded
+      else if (U8.eq reason_code define_disconnect_reason_administrative_action) then
+        define_struct_disconnect_administrative_action
+      else if (U8.eq reason_code define_disconnect_reason_payload_format_invalid) then
+        define_struct_disconnect_payload_format_invalid
+      else if (U8.eq reason_code define_disconnect_reason_retain_not_supported) then
+        define_struct_disconnect_retain_not_supported
+      else if (U8.eq reason_code define_disconnect_reason_qos_not_supported) then
+        define_struct_disconnect_qos_not_supported
+      else if (U8.eq reason_code define_disconnect_reason_use_another_server) then
+        define_struct_disconnect_use_another_server
+      else if (U8.eq reason_code define_disconnect_reason_server_moved) then
+        define_struct_disconnect_server_moved
+      else if (U8.eq reason_code define_disconnect_reason_shared_subscriptions_not_supported) then
+        define_struct_disconnect_shared_subscriptions_not_supported
+      else if (U8.eq reason_code define_disconnect_reason_connection_rate_exceeded) then
+        define_struct_disconnect_connection_rate_exceeded
+      else if (U8.eq reason_code define_disconnect_reason_maximum_connect_time) then
+        define_struct_disconnect_maximum_connect_time
+      else if (U8.eq reason_code define_disconnect_reason_subscription_identifiers_not_supported) then
+        define_struct_disconnect_subscription_identifiers_not_supported
+      else if (U8.eq reason_code define_disconnect_reason_wildcard_subscriptions_not_supported) then
+        define_struct_disconnect_wildcard_subscriptions_not_supported
+      else
+        define_struct_disconnect_error
+    ) in disconnect_reason_struct
+
+val disconnect_packet_parser: packet_data: (B.buffer U8.t) 
+  -> packet_size: type_packet_size 
+  -> next_start_index:U32.t
+  -> Stack (disconnect_packet_seed: struct_disconnect_packet_seed)
+    (requires fun h0 -> B.live h0 packet_data)
+    (ensures fun h0 r h1 -> true)
+let disconnect_packet_parser packet_data packet_size next_start_index =
+  push_frame ();
+  let reason_code_start_index: U32.t = next_start_index in
+  let reason_code: type_disconnect_reason_code = packet_data.(reason_code_start_index) in
+  let disconnect_reason_struct: struct_disconnect_reason = get_disconnect_reason reason_code in
+  let property_start_index: U32.t = U32.add reason_code_start_index 1ul in
+  let property_struct: struct_property = 
+    parse_property packet_data packet_size property_start_index in
+  pop_frame ();
+  let disconnect_packet_seed_struct :struct_disconnect_packet_seed = 
+    {
+      disconnect_seed_reason = disconnect_reason_struct;
+      disconnect_seed_property = property_struct;
+    } in disconnect_packet_seed_struct
+
 val disconnect_packet_parse_result: (share_common_data: struct_share_common_data)
   -> Stack (r: struct_fixed_header)
     (requires fun h0 -> true)
     (ensures fun h0 r h1 -> true)
 let disconnect_packet_parse_result share_common_data =
+  // Reason Code, Property ともに省略
   let disconnect_constant: struct_fixed_header_constant =
     get_struct_fixed_header_constant_except_publish share_common_data.common_message_type in
-  let flag: type_flag_restrict = get_flag share_common_data.common_message_type share_common_data.common_first_one_byte in
-  let have_error: bool =
-    (is_valid_flag disconnect_constant flag = false) in
-    if (have_error) then
-      (
-        let error_struct: struct_error_struct =
-          {
-              code = define_error_flag_invalid_code;
-              message = define_error_flag_invalid;
-          }
-        in error_struct_fixed_header error_struct
-      )
-    else
-      (
-        let ed_fixed_header_parts:
-        struct_disconnect_parts = {
-          disconnect_disconnect_constant = disconnect_constant;
-          disconnect_remaining_length = share_common_data.common_remaining_length;
-        } in
-        assemble_disconnect_struct ed_fixed_header_parts
-      )
+  if (share_common_data.common_remaining_length = 0ul) then
+    (
+      let disconnect_struct: struct_disconnect = {
+        disconnect_reason = define_struct_disconnect_normal_disconnection;
+      } in
+      let ed_fixed_header_parts: struct_disconnect_parts = {
+        disconnect_disconnect_constant = disconnect_constant;
+        disconnect_remaining_length = share_common_data.common_remaining_length;
+        disconnect_struct = disconnect_struct;
+        property = property_struct_base;
+      } in
+      assemble_disconnect_struct ed_fixed_header_parts
+    )
+  else 
+    (
+      let disconnect_packet_seed: struct_disconnect_packet_seed = 
+        disconnect_packet_parser
+          share_common_data.common_packet_data
+          share_common_data.common_packet_size 
+          share_common_data.common_next_start_index in
+      let disconnect_reason: struct_disconnect_reason = disconnect_packet_seed.disconnect_seed_reason in
+      let disconnect_property: struct_property = disconnect_packet_seed.disconnect_seed_property in
+      let have_error: bool =
+        (
+          disconnect_reason.disconnect_reason_code = max_u8 ||
+          U8.gt disconnect_property.property_type_struct.property_type_error.property_error_code 0uy
+        ) in
+        if (have_error) then
+          (
+            let error_struct: struct_error_struct =
+              if (disconnect_reason.disconnect_reason_code = max_u8) then
+                {
+                    code = define_error_disconnect_reason_invalid_code;
+                    message = define_error_disconnect_reason_invalid;
+                }
+              else // if (U8.gt disconnect_property.property_type_struct.property_type_error.property_error_code 0uy) then
+                {
+                  code = define_error_property_error_code;
+                  message = disconnect_property.property_type_struct.property_type_error.property_error_code_name;
+                }
+            in error_struct_fixed_header error_struct
+          )
+        else
+          (
+            let disconnect_struct: struct_disconnect = {
+              disconnect_reason = disconnect_reason;
+            } in
+            let ed_fixed_header_parts:
+            struct_disconnect_parts = {
+              disconnect_disconnect_constant = disconnect_constant;
+              disconnect_remaining_length = share_common_data.common_remaining_length;
+              disconnect_struct = disconnect_struct;
+              property = disconnect_property;
+            } in
+            assemble_disconnect_struct ed_fixed_header_parts
+          )
+    )
