src/mqtt-packet-parser/src/publish.fst
@@ -1,6 +1,7 @@
 module Publish
 
 module U8 = FStar.UInt8
+module U16 = FStar.UInt16
 module U32 = FStar.UInt32
 module B = LowStar.Buffer
 
@@ -17,7 +18,7 @@ open Debug_FFI
 
 val get_dup_flag: fixed_header_first_one_byte: U8.t -> type_dup_flags_restrict
 let get_dup_flag fixed_header_first_one_byte =
-  let dup_flag_bits: U8.t = slice_byte fixed_header_first_one_byte 4uy 5uy in
+  let dup_flag_bits: U8.t = slice_byte fixed_header_first_one_byte 0uy 1uy in
   if (U8.gt dup_flag_bits 1uy) then
     max_u8
   else
@@ -25,7 +26,7 @@ let get_dup_flag fixed_header_first_one_byte =
 
 val get_qos_flag: fixed_header_first_one_byte: U8.t -> type_qos_flags_restrict
 let get_qos_flag fixed_header_first_one_byte =
-    let qos_flag_bits: U8.t = slice_byte fixed_header_first_one_byte 5uy 7uy in
+    let qos_flag_bits: U8.t = slice_byte fixed_header_first_one_byte 1uy 3uy in
     if (U8.gt qos_flag_bits 2uy) then
       max_u8
     else
@@ -33,22 +34,23 @@ let get_qos_flag fixed_header_first_one_byte =
 
 val get_retain_flag: fixed_header_first_one_byte: U8.t -> type_retain_flags_restrict
 let get_retain_flag fixed_header_first_one_byte =
-    let retain_flag_bits: U8.t = slice_byte fixed_header_first_one_byte 7uy 8uy in
+    let retain_flag_bits: U8.t = slice_byte fixed_header_first_one_byte 3uy 4uy in
     if (U8.gt retain_flag_bits 1uy) then
       max_u8
     else
       retain_flag_bits
 
 val struct_fixed_publish:
-  (dup_flag:type_dup_flags_restrict)
-  -> (qos_flag:type_qos_flags_restrict)
-  -> (retain_flag:type_retain_flags_restrict)
+  flag: type_flag_restrict
+  -> dup_flag:type_dup_flags_restrict
+  -> qos_flag:type_qos_flags_restrict
+  -> retain_flag:type_retain_flags_restrict
   -> struct_fixed_header_constant
-let struct_fixed_publish dup_flag qos_flag retain_flag = {
+let struct_fixed_publish flag dup_flag qos_flag retain_flag = {
   message_type_constant = define_mqtt_control_packet_PUBLISH;
   message_name_constant = define_mqtt_control_packet_PUBLISH_label;
   flags_constant = {
-    flag = max_u8;
+    flag = flag;
     dup_flag = dup_flag;
     qos_flag = qos_flag;
     retain_flag = retain_flag;
@@ -60,11 +62,12 @@ val assemble_publish_struct: s: struct_publish_parts
     (requires fun h0 -> true)
     (ensures fun h0 r h1 -> true)
 let assemble_publish_struct s =
-  let dup_flag: type_dup_flags_restrict = get_dup_flag s.publish_fixed_header_first_one_byte in
-  let qos_flag: type_qos_flags_restrict = get_qos_flag s.publish_fixed_header_first_one_byte in
-  let retain_flag: type_retain_flags_restrict = get_retain_flag s.publish_fixed_header_first_one_byte in
+  // let dup_flag: type_dup_flags_restrict = get_dup_flag s.publish_fixed_header_first_one_byte in
+  // let qos_flag: type_qos_flags_restrict = get_qos_flag s.publish_fixed_header_first_one_byte in
+  // let retain_flag: type_retain_flags_restrict = get_retain_flag s.publish_fixed_header_first_one_byte in
   let data: struct_fixed_header_constant =
-    struct_fixed_publish dup_flag qos_flag retain_flag in
+    struct_fixed_publish 
+      s.publish_flag s.publish_dup_flag s.publish_qos_flag s.publish_retain_flag in
     {
       message_type = data.message_type_constant;
       message_name = data.message_name_constant;
@@ -99,14 +102,17 @@ let assemble_publish_struct s =
       publish = {
         topic_length = s.publish_topic_length;
         topic_name = s.publish_topic_name;
+        packet_identifier = s.publish_packet_identifier;
         property_length = s.publish_property_length;
         property_id = s.publish_property_id;
         payload = s.publish_payload;
         payload_length = s.publish_payload_length;
       };
       disconnect = {
-        disconnect_reason_code = max_u8;
-        disconnect_reason_code_name = !$"";
+        disconnect_reason = {
+          disconnect_reason_code = max_u8;
+          disconnect_reason_code_name = !$"";
+        };
       };
       property = s.publish_property;
       error = {
@@ -180,13 +186,18 @@ let get_topic_name packet_data topic_name_start_index topic_length =
 
 val publish_packet_parser: packet_data: (B.buffer U8.t) 
   -> packet_size: type_packet_size 
+  -> common_flag: type_flag_restrict
   -> next_start_index:U32.t
   -> Stack (publish_packet_seed: struct_publish_packet_seed)
     (requires fun h0 -> B.live h0 packet_data)
     (ensures fun h0 r h1 -> true)
-let publish_packet_parser packet_data packet_size next_start_index =
+let publish_packet_parser packet_data packet_size common_flag next_start_index =
   push_frame();
+  let dup_flag: type_dup_flags_restrict = get_dup_flag common_flag in
+  let qos_flag: type_qos_flags_restrict = get_qos_flag common_flag in
+  let retain_flag: type_retain_flags_restrict = get_retain_flag common_flag in
 
+  // TODO: topic name のリファクタ
   let msb_u8: U8.t = packet_data.(next_start_index) in
   let lsb_u8: U8.t = packet_data.(U32.add next_start_index 1ul) in
   let msb_u32: U32.t = uint8_to_uint32 msb_u8  in
@@ -198,9 +209,33 @@ let publish_packet_parser packet_data packet_size next_start_index =
     get_topic_name packet_data (U32.add next_start_index 2ul) topic_length in
   let topic_name_error_status: U8.t = topic_name_struct.topic_name_error_status in
 
+  let packet_identifier_struct: struct_packet_identifier = 
+    (
+      if (U8.gt qos_flag 0uy) then
+        (
+          let packet_identifier_value: U16.t = 
+            get_two_byte_integer_u8_to_u16 
+              packet_data.(U32.add (U32.add next_start_index 2ul) topic_length)
+              packet_data.(U32.add (U32.add next_start_index 3ul) topic_length) in
+            let packet_identifier_struct :struct_packet_identifier = 
+              {
+                packet_identifier_value = packet_identifier_value;
+                property_start_to_offset = 2ul;
+              } in packet_identifier_struct
+        )
+      else 
+        (
+          let packet_identifier_struct: struct_packet_identifier = 
+            {
+              packet_identifier_value = max_u16;
+              property_start_to_offset = 0ul;
+            } in packet_identifier_struct
+        )
+    ) in
+
   // TODO: propertyが存在しない場合の処理
   let property_start_index: U32.t = 
-    (U32.add (U32.add next_start_index 2ul) topic_length) in
+    U32.(next_start_index +^ 2ul +^ topic_length +^ packet_identifier_struct.property_start_to_offset) in
   let property_struct: struct_property = 
     parse_property packet_data packet_size property_start_index in
   let property_id = property_struct.property_id in
@@ -222,9 +257,13 @@ let publish_packet_parser packet_data packet_size next_start_index =
   
 
   let publish_packet_seed: struct_publish_packet_seed = {
+    publish_seed_dup_flag = dup_flag;
+    publish_seed_qos_flag = qos_flag;
+    publish_seed_retain_flag = retain_flag;
     publish_seed_topic_length = topic_length;
     publish_seed_topic_name = topic_name_struct.topic_name;
     publish_seed_topic_name_error_status = topic_name_error_status;
+    publish_seed_packet_identifier = packet_identifier_struct.packet_identifier_value;
     publish_seed_is_searching_property_length = false;
     publish_seed_property_length = 0ul;
     publish_seed_payload = 
@@ -241,17 +280,17 @@ val publish_packet_parse_result: (share_common_data: struct_share_common_data)
     (ensures fun h0 r h1 -> true)
 let publish_packet_parse_result share_common_data =
   let publish_packet_seed: struct_publish_packet_seed = 
-    publish_packet_parser share_common_data.common_packet_data share_common_data.common_packet_size share_common_data.common_next_start_index in
-  let first_one_byte: U8.t = share_common_data.common_first_one_byte in
-  let dup_flag: type_dup_flags_restrict = get_dup_flag first_one_byte in
-  let qos_flag: type_qos_flags_restrict = get_qos_flag first_one_byte in
-  let retain_flag: type_retain_flags_restrict = get_retain_flag first_one_byte in
+    publish_packet_parser 
+      share_common_data.common_packet_data
+      share_common_data.common_packet_size
+      share_common_data.common_flag
+      share_common_data.common_next_start_index in
   // TODO: エラーコードの見直し
   // Poroperty_error
   let have_error: bool =
-    (U8.eq dup_flag max_u8) ||
-    (U8.eq qos_flag max_u8) ||
-    (U8.eq retain_flag max_u8) ||
+    (U8.eq publish_packet_seed.publish_seed_dup_flag max_u8) ||
+    (U8.eq publish_packet_seed.publish_seed_qos_flag max_u8) ||
+    (U8.eq publish_packet_seed.publish_seed_retain_flag max_u8) ||
     (U32.eq publish_packet_seed.publish_seed_topic_length max_u32) ||
     (U8.eq publish_packet_seed.publish_seed_topic_name_error_status 1uy) ||
     (U8.eq publish_packet_seed.publish_seed_topic_name_error_status 2uy) ||
@@ -262,17 +301,17 @@ let publish_packet_parse_result share_common_data =
     (
       let error_struct: struct_error_struct =
         (
-          if (U8.eq dup_flag max_u8) then
+          if (U8.eq publish_packet_seed.publish_seed_dup_flag max_u8) then
             {
               code = define_error_dup_flag_invalid_code;
               message = define_error_dup_flag_invalid;
             }
-          else if (U8.eq qos_flag max_u8) then
+          else if (U8.eq publish_packet_seed.publish_seed_qos_flag max_u8) then
             {
               code = define_error_qos_flag_invalid_code;
               message = define_error_qos_flag_invalid;
             }
-          else if (U8.eq retain_flag max_u8) then
+          else if (U8.eq publish_packet_seed.publish_seed_retain_flag max_u8) then
             {
               code = define_error_retain_flag_invalid_code;
               message = define_error_retain_flag_invalid;
@@ -309,10 +348,14 @@ let publish_packet_parse_result share_common_data =
     (
       let ed_fixed_header_parts:
         struct_publish_parts = {
-          publish_fixed_header_first_one_byte = first_one_byte;
+          publish_flag = share_common_data.common_flag;
+          publish_dup_flag = publish_packet_seed.publish_seed_dup_flag;
+          publish_qos_flag = publish_packet_seed.publish_seed_qos_flag;
+          publish_retain_flag = publish_packet_seed.publish_seed_retain_flag;
           publish_remaining_length = share_common_data.common_remaining_length;
           publish_topic_length = publish_packet_seed.publish_seed_topic_length;
           publish_topic_name = publish_packet_seed.publish_seed_topic_name;
+          publish_packet_identifier = publish_packet_seed.publish_seed_packet_identifier;
           publish_property_length = publish_packet_seed.publish_seed_property_length;
           publish_payload = publish_packet_seed.publish_seed_payload;
           publish_payload_length = publish_packet_seed.publish_seed_payload_length;
